Merging in fabian's changes

src/coq/players.v
@@ -6,3 +6,7 @@ Include ListNotations.
 Load "_players/naive".
 Load "_players/intelligent".
 
+(*
+Definition player:= (macro_board -> move -> move).
+Example p1: player:= intelligent_player.
+*)
